finish ule

src/BitBlastingSimple.v
@@ -4082,6 +4082,12 @@ Definition bit_blast_ule (w: nat) g (ls1 ls2: w.-tuple literal) : generator * cn
   let '(g_disj, cs_disj, r_disj) := bit_blast_disj g_ult r_eq r_ult in
   (g_disj, cs_eq++cs_ult++cs_disj, r_disj).
 
+Definition mk_env_ule w E g (ls1 ls2: w.-tuple literal) : env * generator * cnf * literal :=
+  let '(E_eq, g_eq, cs_eq, r_eq) := mk_env_eq E g ls1 ls2 in
+  let '(E_ult, g_ult, cs_ult, r_ult) := mk_env_ult E_eq g_eq ls1 ls2 in
+  let '(E_disj, g_disj, cs_disj, r_disj) := mk_env_disj E_ult g_ult r_eq r_ult in
+  (E_disj, g_disj, cs_eq++cs_ult++cs_disj, r_disj).
+
 Lemma bit_blast_ule_correct :
   forall w g (bs1 bs2 : BITS w) E g' ls1 ls2 cs lr,
     bit_blast_ule g ls1 ls2 = (g', cs, lr) ->
@@ -4105,6 +4111,143 @@ Proof.
   move : (bit_blast_disj_correct Hdisj Hreq Hrult Hcnf_disj) => Hrdisj.
   rewrite /enc_bit in Hrdisj. move/eqP: Hrdisj => Hrdisj.
   apply/eqP; by rewrite /leB/enc_bit Bool.orb_comm.
+Qed.
+
+Lemma mk_env_ule_is_bit_blast_ule :
+  forall w E g (ls1 ls2 : w.-tuple literal) E' g' cs lrs,
+    mk_env_ule E g ls1 ls2 = (E', g', cs, lrs) ->
+    bit_blast_ule g ls1 ls2 = (g', cs, lrs).
+Proof.
+  rewrite /bit_blast_ule /mk_env_ule /= => w E g ls1 ls2 E' g' cs lrs.
+  move => H. dcase_hyps. subst.
+  rewrite (mk_env_eq_is_bit_blast_eq H).
+  rewrite (mk_env_ult_is_bit_blast_ult H1).
+  done.
+Qed.
+
+Lemma mk_env_ule_newer_gen :
+  forall w E g (ls1 ls2: w.-tuple literal) E' g' cs lr,
+    mk_env_ule E g ls1 ls2 = (E', g', cs, lr) ->
+    (g <=? g')%positive.
+Proof.
+  move=> w E g ls1 ls2 E' g' cs lr. rewrite /mk_env_ule. rewrite /gen.
+  case Heq: (mk_env_eq E g ls1 ls2) => [[[E_eq g_eq] cs_eq] lr_eq].
+  case Hult: (mk_env_ult E_eq g_eq ls1 ls2) => [[[E_ult g_ult] cs_ult] lr_ult].
+  case Hdisj: (mk_env_disj E_ult g_ult lr_eq lr_ult) => [[[E_disj g_disj] cs_disj] lr_disj].
+  case. move=> _ <- _ _ .
+  move: (mk_env_disj_newer_gen Hdisj) => g_ult_le_g_disj.
+  move: (mk_env_ult_newer_gen Hult) => g_eq_le_g_ult.
+  move: (mk_env_eq_newer_gen Heq) => g_le_g_eq.
+  apply: (pos_leb_trans (pos_leb_trans g_le_g_eq g_eq_le_g_ult) g_ult_le_g_disj).
+Qed.
+
+Lemma mk_env_ule_newer_res :
+  forall w E g (ls1 ls2: w.-tuple literal) E' g' cs lr,
+    mk_env_ule E g ls1 ls2 = (E', g', cs, lr) ->
+    newer_than_lit g' lr.
+Proof.
+  move=> w E g ls1 ls2 E' g' cs lr. rewrite /mk_env_ule. rewrite /gen.
+  case Heq: (mk_env_eq E g ls1 ls2) => [[[E_eq g_eq] cs_eq] lr_eq].
+  case Hult: (mk_env_ult E_eq g_eq ls1 ls2) => [[[E_ult g_ult] cs_ult] lr_ult].
+  case Hdisj: (mk_env_disj E_ult g_ult lr_eq lr_ult) => [[[E_disj g_disj] cs_disj] lr_disj].
+  case. move=> _ <- _ <-.
+  exact: (mk_env_disj_newer_res Hdisj).
+Qed.
+
+Lemma mk_env_ule_newer_cnf :
+forall w E g (ls1 ls2 : w.-tuple literal) E' g' cs lr,
+  mk_env_ule E g ls1 ls2 = (E', g', cs, lr) ->
+  newer_than_lits g ls1 -> newer_than_lits g ls2 ->
+  newer_than_cnf g' cs.
+Proof.
+  move=> w E g ls1 ls2 E' g' cs lr. rewrite /mk_env_ule. rewrite /gen.
+  case Heq: (mk_env_eq E g ls1 ls2) => [[[E_eq g_eq] cs_eq] lr_eq].
+  case Hult: (mk_env_ult E_eq g_eq ls1 ls2) => [[[E_ult g_ult] cs_ult] lr_ult].
+  case Hdisj: (mk_env_disj E_ult g_ult lr_eq lr_ult) => [[[E_disj g_disj] cs_disj] lr_disj].
+  case. move=> _ <- <- _. move=> Hnew_gls1 Hnew_gls2.
+  rewrite 2!newer_than_cnf_append.
+  move: (mk_env_eq_newer_cnf Heq Hnew_gls1 Hnew_gls2) => H_new_cnf_geq_cseq.
+  move: (mk_env_eq_newer_gen Heq) => g_le_geq.
+  move: (mk_env_ult_newer_gen Hult) => geq_le_gult.
+  move: (newer_than_lits_le_newer Hnew_gls1 g_le_geq) => Hnew_geqls1.
+  move: (newer_than_lits_le_newer Hnew_gls2 g_le_geq) => Hnew_geqls2.
+  move: (mk_env_ult_newer_cnf Hult Hnew_geqls1 Hnew_geqls2) => H_new_cnf_gult_csult.
+  move: (mk_env_disj_newer_res Hdisj) => tmp.
+  move: (mk_env_ult_newer_res Hult) => tmp2.
+  move: (mk_env_eq_newer_res Heq) => tmp3.
+  move: (newer_than_lit_le_newer tmp3 geq_le_gult) => tmp4.
+  move: (mk_env_disj_newer_cnf Hdisj tmp4 tmp2) => -> /=.
+  move: (mk_env_disj_newer_gen Hdisj) => g_ult_le_g_disj.
+  move: (newer_than_cnf_le_newer H_new_cnf_gult_csult g_ult_le_g_disj) => -> /=.
+  move: (pos_leb_trans geq_le_gult g_ult_le_g_disj) => geq_le_gdisj.
+  move: (newer_than_cnf_le_newer H_new_cnf_geq_cseq geq_le_gdisj) => -> /=.
+  done.
+Qed.
+
+
+Lemma mk_env_ule_preserve :
+  forall w E g (ls1 ls2 : w.-tuple literal) E' g' cs lr,
+    mk_env_ule E g ls1 ls2 = (E', g', cs, lr) ->
+    env_preserve E E' g.
+Proof.
+  move=> w E g ls1 ls2 E' g' cs lr. rewrite /mk_env_ule. rewrite /gen.
+  case Heq: (mk_env_eq E g ls1 ls2) => [[[E_eq g_eq] cs_eq] lr_eq].
+  case Hult: (mk_env_ult E_eq g_eq ls1 ls2) => [[[E_ult g_ult] cs_ult] lr_ult].
+  case Hdisj: (mk_env_disj E_ult g_ult lr_eq lr_ult) => [[[E_disj g_disj] cs_disj] lr_disj].
+  case=> <- _ _ _.
+  move: (mk_env_eq_preserve Heq) => Hpre_eq.
+  move: (mk_env_ult_preserve Hult) => Hpre_ult.
+  move: (mk_env_disj_preserve Hdisj) => Hpre_disj.
+  move: (mk_env_eq_newer_gen Heq) => Hng_eq.
+  move: (mk_env_ult_newer_gen Hult) => Hng_ult.
+  move: (mk_env_disj_newer_gen Hdisj) => Hng_disj.
+  move: (env_preserve_le Hpre_ult Hng_eq) => Hpre2.
+  move: (pos_leb_trans Hng_eq Hng_ult) => g_le_gult.
+  move: (env_preserve_le Hpre_disj g_le_gult) => Hpre3.
+  exact: (env_preserve_trans (env_preserve_trans Hpre_eq Hpre2) Hpre3).
+Qed.
+
+
+Lemma mk_env_ule_sat :
+  forall w E g (ls1 ls2 : w.-tuple literal) E' g' cs lr,
+    mk_env_ule E g ls1 ls2 = (E', g', cs, lr) ->
+    newer_than_lits g ls1 -> newer_than_lits g ls2 ->
+    interp_cnf E' cs.
+Proof.
+  move=> w E g ls1 ls2 E' g' cs lr. rewrite /mk_env_ule. rewrite /gen.
+  case Heq: (mk_env_eq E g ls1 ls2) => [[[E_eq g_eq] cs_eq] lr_eq].
+  case Hult: (mk_env_ult E_eq g_eq ls1 ls2) => [[[E_ult g_ult] cs_ult] lr_ult].
+  case Hdisj: (mk_env_disj E_ult g_ult lr_eq lr_ult) => [[[E_disj g_disj] cs_disj] lr_disj].
+  case=> <- _ <- _. move=> Hnew_gls1 Hnew_gls2.
+  rewrite 2!interp_cnf_append.
+  move: (mk_env_eq_newer_cnf Heq Hnew_gls1 Hnew_gls2) => H_new_cnf_geq_cseq.
+  move: (mk_env_eq_newer_gen Heq) => g_le_geq.
+  move: (mk_env_ult_newer_gen Hult) => geq_le_gult.
+  move: (newer_than_lits_le_newer Hnew_gls1 g_le_geq) => Hnew_geqls1.
+  move: (newer_than_lits_le_newer Hnew_gls2 g_le_geq) => Hnew_geqls2.
+  move: (mk_env_ult_sat Hult Hnew_geqls1 Hnew_geqls2) => Hsat_ult.
+  move: (mk_env_disj_newer_gen Hdisj) => g_ult_le_g_disj.
+  move: (mk_env_disj_preserve Hdisj) => Hpre_disj.
+  move: (newer_than_lits_le_newer Hnew_geqls1 geq_le_gult) => Hnew_gultls1.
+  move: (newer_than_lits_le_newer Hnew_geqls2 geq_le_gult) => Hnew_gultls2.
+  move: (mk_env_ult_newer_cnf Hult Hnew_geqls1 Hnew_geqls2) => Hnew_cnf_gult_csult.
+  move: (env_preserve_cnf Hpre_disj Hnew_cnf_gult_csult) => -> /=.
+  rewrite Hsat_ult /=.
+  move: (mk_env_disj_newer_res Hdisj) => tmp.
+  move: (mk_env_ult_newer_res Hult) => tmp2.
+  move: (mk_env_eq_newer_res Heq) => tmp3.
+  move: (newer_than_lit_le_newer tmp3 geq_le_gult) => tmp4.
+  move: (mk_env_disj_sat Hdisj tmp4 tmp2) => -> /=.
+  move: (mk_env_eq_sat Heq Hnew_gls1 Hnew_gls2) => H.
+  move: (mk_env_eq_preserve Heq) => Hpre_eq.
+  move: (mk_env_ult_preserve Hult) => Hpre_ult.
+  move: (mk_env_eq_newer_cnf Heq Hnew_gls1 Hnew_gls2) => Hnew_cnf_geq_cseq.
+  move: (env_preserve_cnf Hpre_ult Hnew_cnf_geq_cseq) => eq1.
+  rewrite H in eq1.
+  move: (mk_env_disj_newer_cnf Hdisj tmp4 tmp2) => Hnew_cnf_gdisj_csdisj.
+  move: (newer_than_cnf_le_newer Hnew_cnf_geq_cseq geq_le_gult) => Hnewcnf_gult_cseq.
+  move: (env_preserve_cnf Hpre_disj Hnewcnf_gult_cseq) => -> /=.
+  by rewrite eq1 /=.
 Qed.
 
 (* ===== bit_blast_ugt ===== *)
@@ -5114,7 +5257,11 @@ bit_blast_bexp (m : vm) (g : generator) (e : QFBV64.bexp) : vm * generator * cnf
     let '(m2, g2, cs2, ls2) := bit_blast_exp m1 g1 e2 in
     let '(g', cs, r) := bit_blast_ult g2 ls1 ls2 in
     (m2, g', cs1++cs2++cs, r)
-  | QFBV64.bvUle w e1 e2 => (m, g, [], lit_ff) (* TODO *)
+  | QFBV64.bvUle w e1 e2 =>
+    let '(m1, g1, cs1, ls1) := bit_blast_exp m g e1 in
+    let '(m2, g2, cs2, ls2) := bit_blast_exp m1 g1 e2 in
+    let '(g', cs, r) := bit_blast_ule g2 ls1 ls2 in
+    (m2, g', cs1++cs2++cs, r)
   | QFBV64.bvUgt w e1 e2 => (m, g, [], lit_ff) (* TODO *)
   | QFBV64.bvUge w e1 e2 => (m, g, [], lit_ff) (* TODO *)
   | QFBV64.bvSlt w e1 e2 => (m, g, [], lit_ff) (* TODO *)
@@ -5242,7 +5389,11 @@ mk_env_bexp (m : vm) (s : QFBV64.State.t) (E : env) (g : generator) (e : QFBV64.
     let '(m2, E2, g2, cs2, ls2) := mk_env_exp m1 s E1 g1 e2 in
     let '(E', g', cs, r) := mk_env_ult E2 g2 ls1 ls2 in
     (m2, E', g', cs1++cs2++cs, r)
-  | QFBV64.bvUle w e1 e2 => (m, E, g, [], lit_ff) (* TODO *)
+  | QFBV64.bvUle w e1 e2 =>
+    let '(m1, E1, g1, cs1, ls1) := mk_env_exp m s E g e1 in
+    let '(m2, E2, g2, cs2, ls2) := mk_env_exp m1 s E1 g1 e2 in
+    let '(E', g', cs, r) := mk_env_ule E2 g2 ls1 ls2 in
+    (m2, E', g', cs1++cs2++cs, r)
   | QFBV64.bvUgt w e1 e2 => (m, E, g, [], lit_ff) (* TODO *)
   | QFBV64.bvUge w e1 e2 => (m, E, g, [], lit_ff) (* TODO *)
   | QFBV64.bvSlt w e1 e2 => (m, E, g, [], lit_ff) (* TODO *)
@@ -5632,9 +5783,6 @@ Proof.
 Qed.
 
 Lemma bit_blast_bexp_preserve_ult :
-  (* forall (w : nat) (e e0 : QFBV64.exp w) (m : vm) (g : generator) *)
-  (*        (m' : vm) (g' : generator) (cs : cnf) (lrs : literal), *)
-  (*   bit_blast_bexp m g (QFBV64.bvUlt w e e0) = (m', g', cs, lrs) -> vm_preserve m m'. *)
   forall (w : nat) (e1 : QFBV64.exp w)
          (IH1 : forall (m : vm) (g : generator)
                        (m' : vm) (g' : generator) (cs : cnf) (lrs : w.-tuple literal),
@@ -5653,11 +5801,22 @@ Proof.
 Qed.
 
 Lemma bit_blast_bexp_preserve_ule :
- forall (w : nat) (e e0 : QFBV64.exp w) (m : vm) (g : generator)
-        (m' : vm) (g' : generator) (cs : cnf) (lrs : literal),
-   bit_blast_bexp m g (QFBV64.bvUle w e e0) = (m', g', cs, lrs) -> vm_preserve m m'.
+  forall (w : nat) (e1 : QFBV64.exp w)
+         (IH1 : forall (m : vm) (g : generator)
+                       (m' : vm) (g' : generator) (cs : cnf) (lrs : w.-tuple literal),
+             bit_blast_exp m g e1 = (m', g', cs, lrs) ->
+             vm_preserve m m')
+         (e2 : QFBV64.exp w)
+         (IH2 : forall (m : vm) (g : generator)
+                       (m' : vm) (g' : generator) (cs : cnf) (lrs : w.-tuple literal),
+             bit_blast_exp m g e2 = (m', g', cs, lrs) ->
+             vm_preserve m m')
+         (m : vm) (g : generator)
+         (m' : vm) (g' : generator) (cs : cnf) (lrs : literal),
+    bit_blast_bexp m g (QFBV64.bvUle w e1 e2) = (m', g', cs, lrs) -> vm_preserve m m'.
 Proof.
-Admitted.
+  auto_bit_blast_vm_preserve.
+Qed.
 
 Lemma bit_blast_bexp_preserve_ugt :
  forall (w : nat) (e e0 : QFBV64.exp w) (m : vm) (g : generator)
@@ -5876,7 +6035,9 @@ Proof.
   - move=> w e1 e2.
     move: (bit_blast_exp_preserve w e1) (bit_blast_exp_preserve w e2) => IH1 IH2.
     exact: (bit_blast_bexp_preserve_ult IH1 IH2).
-  - exact: bit_blast_bexp_preserve_ule.
+  - move=> w e1 e2.
+    move: (bit_blast_exp_preserve w e1) (bit_blast_exp_preserve w e2) => IH1 IH2.
+    exact: (bit_blast_bexp_preserve_ule IH1 IH2).
   - exact: bit_blast_bexp_preserve_ugt.
   - exact: bit_blast_bexp_preserve_uge.
   - exact: bit_blast_bexp_preserve_slt.
@@ -6555,15 +6716,43 @@ Proof.
 Qed.
 
 Lemma bit_blast_bexp_ule :
-  forall (w : nat) (e e0 : QFBV64.exp w) (m : vm) (g : generator)
-         (s : QFBV64.State.t) (E : env)
+  forall (w : nat)
+         (e : QFBV64.exp w)
+         (IH : forall (m : vm) (g : generator) (s : QFBV64.State.t) (E : env)
+                      (m' : vm) (g' : generator) (cs : cnf) (lrs : w.-tuple literal),
+             bit_blast_exp m g e = (m', g', cs, lrs) ->
+             consistent m' E s ->
+             interp_cnf E (add_prelude cs) ->
+             enc_bits E lrs (QFBV64.eval_exp e s))
+         (e0 : QFBV64.exp w)
+         (IH0 : forall (m : vm) (g : generator) (s : QFBV64.State.t) (E : env)
+                       (m' : vm) (g' : generator) (cs : cnf) (lrs : w.-tuple literal),
+             bit_blast_exp m g e0 = (m', g', cs, lrs) ->
+             consistent m' E s ->
+             interp_cnf E (add_prelude cs) ->
+             enc_bits E lrs (QFBV64.eval_exp e0 s))
+         (m : vm) (g : generator) (s : QFBV64.State.t) (E : env)
          (m' : vm) (g' : generator) (cs : cnf) (lr : literal),
     bit_blast_bexp m g (QFBV64.bvUle w e e0) = (m', g', cs, lr) ->
     consistent m' E s ->
     interp_cnf E (add_prelude cs) ->
     enc_bit E lr (QFBV64.eval_bexp (QFBV64.bvUle w e e0) s).
 Proof.
-Admitted.
+  move=> w e1 IH1 e2 IH2 im ig s E om og ocs olrs.
+  rewrite (lock interp_cnf) /= -lock.
+  case Hblast1: (bit_blast_exp im ig e1) => [[[m1 g1] cs1] rs1].
+  case Hblast2: (bit_blast_exp m1 g1 e2) => [[[m2 g2] cs2] rs2].
+  case Hblastule: (bit_blast_ule g2 rs1 rs2) => [[gule csule] rule].
+  case => Hom Hog Hocs Holrs Hcon Hcs. rewrite -Hocs in Hcs => {Hocs ocs}.
+  rewrite Hog in Hblastule => {Hog gule}. rewrite Hom in Hblast2 => {Hom m2}.
+  rewrite Holrs in Hblastule => {Holrs rule}.
+  rewrite 2!add_prelude_append in Hcs. move/andP: Hcs => [Hcs1 Hcs].
+  move/andP: Hcs => [Hcs2 Hcsule].
+  move: (vm_preserve_consistent (bit_blast_exp_preserve Hblast2) Hcon) => Hcon'.
+  move: (IH1 _ _ _ _ _ _ _ _ Hblast1 Hcon' Hcs1) => Henc1.
+  move: (IH2 _ _ _ _ _ _ _ _ Hblast2 Hcon Hcs2) => Henc2.
+  exact: (bit_blast_ule_correct Hblastule Henc1 Henc2 Hcsule).
+Qed.
 
 Lemma bit_blast_bexp_ugt :
   forall (w : nat) (e e0 : QFBV64.exp w) (m : vm) (g : generator)
@@ -6698,13 +6887,6 @@ Proof.
 Admitted.
 
 Lemma bit_blast_bexp_lneg :
-  (* forall (b : QFBV64.bexp) (m : vm) (g : generator) *)
-  (*        (s : QFBV64.State.t) (E : env) *)
-  (*        (m' : vm) (g' : generator) (cs : cnf) (lr : literal), *)
-  (*   bit_blast_bexp m g (QFBV64.bvLneg b) = (m', g', cs, lr) -> *)
-  (*   consistent m' E s -> *)
-  (*   interp_cnf E (add_prelude cs) -> *)
-  (*   enc_bit E lr (QFBV64.eval_bexp (QFBV64.bvLneg b) s). *)
   forall (b : QFBV64.bexp)
          (IH : forall (m : vm) (g : generator) (s : QFBV64.State.t) (E : env)
                       (m' : vm) (g' : generator) (cs : cnf) (lr : literal),
@@ -6765,13 +6947,6 @@ Proof.
 Qed.
 
 Lemma bit_blast_bexp_disj :
-(*  forall (b b0 : QFBV64.bexp) (m : vm) (g : generator)
-         (s : QFBV64.State.t) (E : env)
-         (m' : vm) (g' : generator) (cs : cnf) (lr : literal),
-    bit_blast_bexp m g (QFBV64.bvDisj b b0) = (m', g', cs, lr) ->
-    consistent m' E s ->
-    interp_cnf E (add_prelude cs) ->
-    enc_bit E lr (QFBV64.eval_bexp (QFBV64.bvDisj b b0) s).*)
   forall (b : QFBV64.bexp)
          (IH : forall (m : vm) (g : generator) (s : QFBV64.State.t) (E : env)
                       (m' : vm) (g' : generator) (cs : cnf) (lr : literal),
@@ -6880,7 +7055,9 @@ Proof.
   - move=> w e1 e2.
     move: (bit_blast_exp_correct _ e1) (bit_blast_exp_correct _ e2) => IH1 IH2.
     exact: (bit_blast_bexp_ult IH1 IH2).
-  - exact: bit_blast_bexp_ule.
+  - move=> w e1 e2.
+    move: (bit_blast_exp_correct _ e1) (bit_blast_exp_correct _ e2) => IH1 IH2.
+    exact: (bit_blast_bexp_ule IH1 IH2).
   - exact: bit_blast_bexp_ugt.
   - exact: bit_blast_bexp_uge.
   - exact: bit_blast_bexp_slt.
@@ -7378,13 +7555,28 @@ Proof.
 Qed.
 
 Lemma mk_env_bexp_is_bit_blast_bexp_ule :
-  forall (w : nat) (e e0 : QFBV64.exp w) (m : vm) (s : QFBV64.State.t)
-         (E : env) (g : generator) (m' : vm) (E' : env) (g' : generator)
-         (cs : cnf) (lr : literal),
-    mk_env_bexp m s E g (QFBV64.bvUle w e e0) = (m', E', g', cs, lr) ->
-    bit_blast_bexp m g (QFBV64.bvUle w e e0) = (m', g', cs, lr).
+  forall (w : nat) (e : QFBV64.exp w),
+    (forall (m : vm) (E : env) (g : generator) (s : QFBV64.State.t)
+            (m' : vm) (E' : env) (g' : generator) (cs : cnf)
+            (lrs : w.-tuple literal),
+        mk_env_exp m s E g e = (m', E', g', cs, lrs) ->
+        bit_blast_exp m g e = (m', g', cs, lrs)) ->
+    forall (e0 : QFBV64.exp w),
+      (forall (m : vm) (E : env) (g : generator) (s : QFBV64.State.t)
+              (m' : vm) (E' : env) (g' : generator) (cs : cnf)
+              (lrs : w.-tuple literal),
+          mk_env_exp m s E g e0 = (m', E', g', cs, lrs) ->
+          bit_blast_exp m g e0 = (m', g', cs, lrs)) ->
+      forall (m : vm) (s : QFBV64.State.t)
+             (E : env) (g : generator) (m' : vm) (E' : env) (g' : generator)
+             (cs : cnf) (lr : literal),
+        mk_env_bexp m s E g (QFBV64.bvUle w e e0) = (m', E', g', cs, lr) ->
+        bit_blast_bexp m g (QFBV64.bvUle w e e0) = (m', g', cs, lr).
 Proof.
-Admitted.
+  rewrite /=; intros; dcase_hyps; subst.
+  rewrite (H _ _ _ _ _ _ _ _ _ H1). rewrite (H0 _ _ _ _ _ _ _ _ _ H3).
+  rewrite (mk_env_ule_is_bit_blast_ule H2). reflexivity.
+Qed.
 
 Lemma mk_env_bexp_is_bit_blast_bexp_ugt :
   forall (w : nat) (e e0 : QFBV64.exp w) (m : vm) (s : QFBV64.State.t)
@@ -7495,11 +7687,6 @@ Proof.
 Admitted.
 
 Lemma mk_env_bexp_is_bit_blast_bexp_lneg :
-  (* forall (b : QFBV64.bexp) (m : vm) (s : QFBV64.State.t) (E : env) *)
-  (*        (g : generator) (m' : vm) (E' : env) (g' : generator) *)
-  (*        (cs : cnf) (lr : literal), *)
-  (*   mk_env_bexp m s E g (QFBV64.bvLneg b) = (m', E', g', cs, lr) -> *)
-  (*   bit_blast_bexp m g (QFBV64.bvLneg b) = (m', g', cs, lr). *)
   forall (b : QFBV64.bexp),
     (forall (m : vm) (s : QFBV64.State.t) (E : env) (g : generator)
             (m' : vm) (E' : env) (g' : generator) (cs : cnf) (lr : literal),
@@ -7537,11 +7724,6 @@ Proof.
 Qed.
 
 Lemma mk_env_bexp_is_bit_blast_bexp_disj :
-(*  forall (b b0 : QFBV64.bexp) (m : vm) (s : QFBV64.State.t)
-         (E : env) (g : generator) (m' : vm) (E' : env) (g' : generator)
-         (cs : cnf) (lr : literal),
-    mk_env_bexp m s E g (QFBV64.bvDisj b b0) = (m', E', g', cs, lr) ->
-    bit_blast_bexp m g (QFBV64.bvDisj b b0) = (m', g', cs, lr).*)
   forall (b : QFBV64.bexp),
     (forall (m : vm) (s : QFBV64.State.t) (E : env) (g : generator)
             (m' : vm) (E' : env) (g' : generator) (cs : cnf) (lr : literal),
@@ -7642,7 +7824,9 @@ Proof.
   - move=> w e1 e2.
     move: (mk_env_exp_is_bit_blast_exp _ e1) (mk_env_exp_is_bit_blast_exp _ e2)
     => IH1 IH2. exact: (mk_env_bexp_is_bit_blast_bexp_ult IH1 IH2).
-  - exact: mk_env_bexp_is_bit_blast_bexp_ule.
+  - move=> w e1 e2.
+    move: (mk_env_exp_is_bit_blast_exp _ e1) (mk_env_exp_is_bit_blast_exp _ e2)
+    => IH1 IH2. exact: (mk_env_bexp_is_bit_blast_bexp_ule IH1 IH2).
   - exact: mk_env_bexp_is_bit_blast_bexp_ugt.
   - exact: mk_env_bexp_is_bit_blast_bexp_uge.
   - exact: mk_env_bexp_is_bit_blast_bexp_slt.
@@ -8137,14 +8321,32 @@ Proof.
   exact: (mk_env_ult_newer_gen Hult).
 Qed.
 
+
 Lemma mk_env_bexp_newer_gen_ule :
-  forall (w : nat) (e e0 : QFBV64.exp w) (m : vm) (s : QFBV64.State.t)
-         (E : env) (g : generator) (m' : vm) (E' : env) (g' : generator)
-         (cs : cnf) (lr : literal),
-    mk_env_bexp m s E g (QFBV64.bvUle w e e0) = (m', E', g', cs, lr) ->
-    (g <=? g')%positive.
+  forall (w : nat) (e : QFBV64.exp w),
+    (forall (m : vm) (s : QFBV64.State.t) (E : env) (g : generator)
+            (m' : vm) (E' : env) (g' : generator) (cs : cnf)
+            (lrs : w.-tuple literal),
+        mk_env_exp m s E g e = (m', E', g', cs, lrs) -> (g <=? g')%positive) ->
+    forall (e0 : QFBV64.exp w),
+      (forall (m : vm) (s : QFBV64.State.t) (E : env) (g : generator)
+              (m' : vm) (E' : env) (g' : generator) (cs : cnf)
+              (lrs : w.-tuple literal),
+          mk_env_exp m s E g e0 = (m', E', g', cs, lrs) -> (g <=? g')%positive) ->
+      forall (m : vm) (s : QFBV64.State.t)
+             (E : env) (g : generator) (m' : vm) (E' : env) (g' : generator)
+             (cs : cnf) (lr : literal),
+        mk_env_bexp m s E g (QFBV64.bvUle w e e0) = (m', E', g', cs, lr) ->
+        (g <=? g')%positive.
 Proof.
-Admitted.
+  move=> w e1 IH1 e2 IH2 m s E g m' E' g' cs lr. rewrite /mk_env_bexp -/mk_env_exp.
+  case Henv1: (mk_env_exp m s E g e1) => [[[[m1 E1] g1] cs1] ls1].
+  case Henv2: (mk_env_exp m1 s E1 g1 e2) => [[[[m2 E2] g2] cs2] ls2].
+  case Hule: (mk_env_ule E2 g2 ls1 ls2)=> [[[oE og] ocs] or].
+  case=> _ _ <- _ _. apply: (pos_leb_trans (IH1 _ _ _ _ _ _ _ _ _ Henv1)).
+  apply: (pos_leb_trans (IH2 _ _ _ _ _ _ _ _ _ Henv2)).
+  exact: (mk_env_ule_newer_gen Hule).
+Qed.
 
 Lemma mk_env_bexp_newer_gen_ugt :
   forall (w : nat) (e e0 : QFBV64.exp w) (m : vm) (s : QFBV64.State.t)
@@ -8255,10 +8457,6 @@ Proof.
 Admitted.
 
 Lemma mk_env_bexp_newer_gen_lneg :
-  (* forall (b : QFBV64.bexp) (m : vm) (s : QFBV64.State.t) (E : env) *)
-  (*        (g : generator) (m' : vm) (E' : env) (g' : generator) *)
-  (*        (cs : cnf) (lr : literal), *)
-  (*   mk_env_bexp m s E g (QFBV64.bvLneg b) = (m', E', g', cs, lr) -> (g <=? g')%positive. *)
   forall (b : QFBV64.bexp),
     (forall (m : vm) (s : QFBV64.State.t) (E : env) (g : generator)
             (m' : vm) (E' : env) (g' : generator) (cs : cnf)
@@ -8305,11 +8503,6 @@ Proof.
 Qed.
 
 Lemma mk_env_bexp_newer_gen_disj :
-(*  forall (b b0 : QFBV64.bexp) (m : vm) (s : QFBV64.State.t)
-         (E : env) (g : generator) (m' : vm) (E' : env) (g' : generator)
-         (cs : cnf) (lr : literal),
-    mk_env_bexp m s E g (QFBV64.bvDisj b b0) = (m', E', g', cs, lr) ->
-    (g <=? g')%positive.*)
   forall (b : QFBV64.bexp),
     (forall (m : vm) (s : QFBV64.State.t) (E : env) (g : generator)
             (m' : vm) (E' : env) (g' : generator) (cs : cnf)
@@ -8407,7 +8600,9 @@ Proof.
   - move=> w e1 e2.
     move: (mk_env_exp_newer_gen _ e1) (mk_env_exp_newer_gen _ e2) => IH1 IH2.
     exact: (mk_env_bexp_newer_gen_ult IH1 IH2).
-  - exact: mk_env_bexp_newer_gen_ule.
+  - move=> w e1 e2.
+    move: (mk_env_exp_newer_gen _ e1) (mk_env_exp_newer_gen _ e2) => IH1 IH2.
+    exact: (mk_env_bexp_newer_gen_ule IH1 IH2).
   - exact: mk_env_bexp_newer_gen_ugt.
   - exact: mk_env_bexp_newer_gen_uge.
   - exact: mk_env_bexp_newer_gen_slt.
@@ -8911,13 +9106,32 @@ Proof.
 Qed.
 
 Lemma mk_env_bexp_newer_vm_ule :
-  forall (w : nat) (e e0 : QFBV64.exp w) (m : vm) (s : QFBV64.State.t)
-         (E : env) (g : generator) (m' : vm) (E' : env) (g' : generator)
-         (cs : cnf) (lr : literal),
-    mk_env_bexp m s E g (QFBV64.bvUle w e e0) = (m', E', g', cs, lr) ->
-    newer_than_vm g m -> newer_than_vm g' m'.
+  forall (w : nat) (e : QFBV64.exp w),
+    (forall (m : vm) (s : QFBV64.State.t) (E : env) (g : generator)
+            (m' : vm) (E' : env) (g' : generator) (cs : cnf)
+            (lrs : w.-tuple literal),
+        mk_env_exp m s E g e = (m', E', g', cs, lrs) ->
+        newer_than_vm g m -> newer_than_vm g' m') ->
+    forall (e0 : QFBV64.exp w),
+      (forall (m : vm) (s : QFBV64.State.t) (E : env) (g : generator)
+              (m' : vm) (E' : env) (g' : generator) (cs : cnf)
+              (lrs : w.-tuple literal),
+          mk_env_exp m s E g e0 = (m', E', g', cs, lrs) ->
+          newer_than_vm g m -> newer_than_vm g' m') ->
+      forall (m : vm) (s : QFBV64.State.t)
+             (E : env) (g : generator) (m' : vm) (E' : env) (g' : generator)
+             (cs : cnf) (lr : literal),
+        mk_env_bexp m s E g (QFBV64.bvUle w e e0) = (m', E', g', cs, lr) ->
+        newer_than_vm g m -> newer_than_vm g' m'.
 Proof.
-Admitted.
+  move=> w e1 IH1 e2 IH2 m s E g m' E' g' cs lr /=.
+  case Henv1: (mk_env_exp m s E g e1) => [[[[m1 E1] g1] cs1] ls1].
+  case Henv2: (mk_env_exp m1 s E1 g1 e2) => [[[[m2 E2] g2] cs2] ls2].
+  case Hule: (mk_env_ule E2 g2 ls1 ls2)=> [[[oE og] ocs] olr]. case=> <- _ <- _ _ Hnew.
+  move: (IH1 _ _ _ _ _ _ _ _ _ Henv1 Hnew) => Hnew1.
+  move: (IH2 _ _ _ _ _ _ _ _ _ Henv2 Hnew1) => Hnew2.
+  apply: (newer_than_vm_le_newer Hnew2). exact: (mk_env_ule_newer_gen Hule).
+Qed.
 
 Lemma mk_env_bexp_newer_vm_ugt :
   forall (w : nat) (e e0 : QFBV64.exp w) (m : vm) (s : QFBV64.State.t)
@@ -9028,11 +9242,6 @@ Proof.
 Admitted.
 
 Lemma mk_env_bexp_newer_vm_lneg :
-  (* forall (b : QFBV64.bexp) (m : vm) (s : QFBV64.State.t) (E : env) *)
-  (*        (g : generator) (m' : vm) (E' : env) (g' : generator) *)
-  (*        (cs : cnf) (lr : literal), *)
-  (*   mk_env_bexp m s E g (QFBV64.bvLneg b) = (m', E', g', cs, lr) -> *)
-  (*   newer_than_vm g m -> newer_than_vm g' m'. *)
   forall (b : QFBV64.bexp),
     (forall (m : vm) (s : QFBV64.State.t) (E : env) (g : generator)
             (m' : vm) (E' : env) (g' : generator) (cs : cnf) (lr : literal),
@@ -9077,11 +9286,6 @@ Proof.
 Qed.
 
 Lemma mk_env_bexp_newer_vm_disj :
-(*  forall (b b0 : QFBV64.bexp) (m : vm) (s : QFBV64.State.t)
-         (E : env) (g : generator) (m' : vm) (E' : env) (g' : generator)
-         (cs : cnf) (lr : literal),
-    mk_env_bexp m s E g (QFBV64.bvDisj b b0) = (m', E', g', cs, lr) ->
-    newer_than_vm g m -> newer_than_vm g' m'.*)
   forall (b : QFBV64.bexp),
     (forall (m : vm) (s : QFBV64.State.t) (E : env) (g : generator)
             (m' : vm) (E' : env) (g' : generator) (cs : cnf) (lr : literal),
@@ -9175,7 +9379,9 @@ Proof.
   - move=> w e1 e2.
     move: (mk_env_exp_newer_vm _ e1) (mk_env_exp_newer_vm _ e2) => IH1 IH2.
     exact: (mk_env_bexp_newer_vm_ult IH1 IH2).
-  - exact: mk_env_bexp_newer_vm_ule.
+  - move=> w e1 e2.
+    move: (mk_env_exp_newer_vm _ e1) (mk_env_exp_newer_vm _ e2) => IH1 IH2.
+    exact: (mk_env_bexp_newer_vm_ule IH1 IH2).
   - exact: mk_env_bexp_newer_vm_ugt.
   - exact: mk_env_bexp_newer_vm_uge.
   - exact: mk_env_bexp_newer_vm_slt.
@@ -9688,6 +9894,7 @@ Proof.
   exact: (mk_env_ult_newer_res H1).
 Qed.
 
+
 Lemma mk_env_bexp_newer_res_ule :
   forall (w : nat) (e e0 : QFBV64.exp w) (m : vm) (s : QFBV64.State.t)
          (E : env) (g : generator) (m' : vm) (E' : env) (g' : generator)
@@ -9695,7 +9902,9 @@ Lemma mk_env_bexp_newer_res_ule :
     mk_env_bexp m s E g (QFBV64.bvUle w e e0) = (m', E', g', cs, lr) ->
     newer_than_lit g lit_tt -> newer_than_lit g' lr.
 Proof.
-Admitted.
+  rewrite /=; intros; dcase_hyps; subst.
+  exact: (mk_env_ule_newer_res H1).
+Qed.
 
 Lemma mk_env_bexp_newer_res_ugt :
   forall (w : nat) (e e0 : QFBV64.exp w) (m : vm) (s : QFBV64.State.t)
@@ -10623,13 +10832,49 @@ Proof.
 Qed.
 
 Lemma mk_env_bexp_newer_cnf_ule :
-  forall (w : nat) (e e0 : QFBV64.exp w) (m : vm) (s : QFBV64.State.t)
-         (E : env) (g : generator) (m' : vm) (E' : env) (g' : generator)
-         (cs : cnf) (lr : literal),
-    mk_env_bexp m s E g (QFBV64.bvUle w e e0) = (m', E', g', cs, lr) ->
-    newer_than_vm g m -> newer_than_lit g lit_tt -> newer_than_cnf g' cs.
+  forall (w : nat) (e : QFBV64.exp w),
+    (forall (m : vm) (s : QFBV64.State.t) (E : env) (g : generator)
+            (m' : vm) (E' : env) (g' : generator) (cs : cnf)
+            (lrs : w.-tuple literal),
+        mk_env_exp m s E g e = (m', E', g', cs, lrs) ->
+        newer_than_vm g m -> newer_than_lit g lit_tt -> newer_than_cnf g' cs) ->
+    forall (e0 : QFBV64.exp w),
+      (forall (m : vm) (s : QFBV64.State.t) (E : env) (g : generator)
+              (m' : vm) (E' : env) (g' : generator) (cs : cnf)
+              (lrs : w.-tuple literal),
+          mk_env_exp m s E g e0 = (m', E', g', cs, lrs) ->
+          newer_than_vm g m -> newer_than_lit g lit_tt -> newer_than_cnf g' cs) ->
+      forall (m : vm) (s : QFBV64.State.t)
+             (E : env) (g : generator) (m' : vm) (E' : env) (g' : generator)
+             (cs : cnf) (lr : literal),
+        mk_env_bexp m s E g (QFBV64.bvUle w e e0) = (m', E', g', cs, lr) ->
+        newer_than_vm g m -> newer_than_lit g lit_tt -> newer_than_cnf g' cs.
 Proof.
-Admitted.
+  move=> w e1 IH1 e2 IH2 m s E g m' E' g' cs lr. rewrite /mk_env_bexp -/mk_env_exp.
+  case Henv1: (mk_env_exp m s E g e1) => [[[[m1 E1] g1] cs1] ls1].
+  case Henv2: (mk_env_exp m1 s E1 g1 e2) => [[[[m2 E2] g2] cs2] ls2].
+  case Hule: (mk_env_ule E2 g2 ls1 ls2)=> [[[oE og] ocs] or].
+  case=> _ _ <- <- _ Hnew_gm Hnew_gtt. rewrite !newer_than_cnf_append.
+  (* newer_than_cnf og cs1 *)
+  move: (IH1 _ _ _ _ _ _ _ _ _ Henv1 Hnew_gm Hnew_gtt) => Hnew_g1cs1.
+  move: (mk_env_exp_newer_gen Henv2) => H_g1g2.
+  move: (newer_than_cnf_le_newer Hnew_g1cs1 H_g1g2) => {Hnew_g1cs1} Hnew_g2cs1.
+  move: (mk_env_ule_newer_gen Hule) => H_g2og.
+  move: (newer_than_cnf_le_newer Hnew_g2cs1 H_g2og) => {Hnew_g2cs1} Hnew_ogcs1.
+  rewrite Hnew_ogcs1 andTb.
+  (* newer_than_cnf og cs2 *)
+  move: (mk_env_exp_newer_vm Henv1 Hnew_gm) => Hnew_g1m1.
+  move: (mk_env_exp_newer_gen Henv1) => H_gg1.
+  move: (newer_than_lit_le_newer Hnew_gtt H_gg1) => Hnew_g1tt.
+  move: (IH2 _ _ _ _ _ _ _ _ _ Henv2 Hnew_g1m1 Hnew_g1tt) => Hnew_g2cs2.
+  move: (newer_than_cnf_le_newer Hnew_g2cs2 H_g2og) => {Hnew_g2cs2} Hnew_ogcs2.
+  rewrite Hnew_ogcs2 andTb.
+  (* newer_than_cnf og ocs *)
+  move: (mk_env_exp_newer_res Henv1 Hnew_gm Hnew_gtt) => Hnew_g1ls1.
+  move: (newer_than_lits_le_newer Hnew_g1ls1 H_g1g2) => {Hnew_g1ls1} Hnew_g2ls1.
+  move: (mk_env_exp_newer_res Henv2 Hnew_g1m1 Hnew_g1tt) => Hnew_g2ls2.
+  exact: (mk_env_ule_newer_cnf Hule Hnew_g2ls1 Hnew_g2ls2).
+Qed.
 
 Lemma mk_env_bexp_newer_cnf_ugt :
   forall (w : nat) (e e0 : QFBV64.exp w) (m : vm) (s : QFBV64.State.t)
@@ -10740,11 +10985,6 @@ Proof.
 Admitted.
 
 Lemma mk_env_bexp_newer_cnf_lneg :
-  (* forall (b : QFBV64.bexp) (m : vm) (s : QFBV64.State.t) (E : env) *)
-  (*        (g : generator) (m' : vm) (E' : env) (g' : generator) *)
-  (*        (cs : cnf) (lr : literal), *)
-  (*   mk_env_bexp m s E g (QFBV64.bvLneg b) = (m', E', g', cs, lr) -> *)
-  (*   newer_than_vm g m -> newer_than_lit g lit_tt -> newer_than_cnf g' cs. *)
   forall (b : QFBV64.bexp),
     (forall (m : vm) (s : QFBV64.State.t) (E : env) (g : generator)
             (m' : vm) (E' : env) (g' : generator) (cs : cnf)
@@ -10818,11 +11058,6 @@ Proof.
 Qed.
 
 Lemma mk_env_bexp_newer_cnf_disj :
-(*  forall (b b0 : QFBV64.bexp) (m : vm) (s : QFBV64.State.t)
-         (E : env) (g : generator) (m' : vm) (E' : env) (g' : generator)
-         (cs : cnf) (lr : literal),
-    mk_env_bexp m s E g (QFBV64.bvDisj b b0) = (m', E', g', cs, lr) ->
-    newer_than_vm g m -> newer_than_lit g lit_tt -> newer_than_cnf g' cs.*)
   forall (b : QFBV64.bexp),
     (forall (m : vm) (s : QFBV64.State.t) (E : env) (g : generator)
             (m' : vm) (E' : env) (g' : generator) (cs : cnf)
@@ -10940,7 +11175,9 @@ Proof.
   - move=> w e1 e2.
     move: (mk_env_exp_newer_cnf _ e1) (mk_env_exp_newer_cnf _ e2) => IH1 IH2.
     exact: (mk_env_bexp_newer_cnf_ult IH1 IH2).
-  - exact: mk_env_bexp_newer_cnf_ule.
+  - move=> w e1 e2.
+    move: (mk_env_exp_newer_cnf _ e1) (mk_env_exp_newer_cnf _ e2) => IH1 IH2.
+    exact: (mk_env_bexp_newer_cnf_ule IH1 IH2).
   - exact: mk_env_bexp_newer_cnf_ugt.
   - exact: mk_env_bexp_newer_cnf_uge.
   - exact: mk_env_bexp_newer_cnf_slt.
@@ -11473,13 +11710,35 @@ Proof.
 Qed.
 
 Lemma mk_env_bexp_consistent_ule :
-  forall (w : nat) (e e0 : QFBV64.exp w) (m : vm) (s : QFBV64.State.t)
-         (E : env) (g : generator) (m' : vm) (E' : env) (g' : generator)
-         (cs : cnf) (lr : literal),
-    mk_env_bexp m s E g (QFBV64.bvUle w e e0) = (m', E', g', cs, lr) ->
-    newer_than_vm g m -> consistent m E s -> consistent m' E' s.
+  forall (w : nat) (e : QFBV64.exp w),
+    (forall (m : vm) (s : QFBV64.State.t) (E : env) (g : generator)
+            (m' : vm) (E' : env) (g' : generator) (cs : cnf)
+            (lrs : w.-tuple literal),
+        mk_env_exp m s E g e = (m', E', g', cs, lrs) ->
+        newer_than_vm g m -> consistent m E s -> consistent m' E' s) ->
+    forall (e0 : QFBV64.exp w),
+      (forall (m : vm) (s : QFBV64.State.t) (E : env) (g : generator)
+              (m' : vm) (E' : env) (g' : generator) (cs : cnf)
+              (lrs : w.-tuple literal),
+          mk_env_exp m s E g e0 = (m', E', g', cs, lrs) ->
+          newer_than_vm g m -> consistent m E s -> consistent m' E' s) ->
+      forall (m : vm) (s : QFBV64.State.t)
+             (E : env) (g : generator) (m' : vm) (E' : env) (g' : generator)
+             (cs : cnf) (lr : literal),
+        mk_env_bexp m s E g (QFBV64.bvUle w e e0) = (m', E', g', cs, lr) ->
+        newer_than_vm g m -> consistent m E s -> consistent m' E' s.
 Proof.
-Admitted.
+  move=> w e1 IH1 e2 IH2 m s E g m' E' g' cs lr. rewrite /mk_env_bexp -/mk_env_exp.
+  case Henv1: (mk_env_exp m s E g e1) => [[[[m1 E1] g1] cs1] ls1].
+  case Henv2: (mk_env_exp m1 s E1 g1 e2) => [[[[m2 E2] g2] cs2] ls2].
+  case Hule: (mk_env_ule E2 g2 ls1 ls2)=> [[[oE og] ocs] or].
+  case=> <- <- _ _ _ Hnew Hcon.
+  move: (mk_env_exp_newer_vm Henv1 Hnew) => Hnew1.
+  move: (mk_env_exp_newer_vm Henv2 Hnew1) => Hnew2.
+  apply: (env_preserve_consistent Hnew2 (mk_env_ule_preserve Hule)).
+  apply: (IH2 _ _ _ _ _ _ _ _ _ Henv2 Hnew1).
+  exact: (IH1 _ _ _ _ _ _ _ _ _ Henv1 Hnew).
+Qed.
 
 Lemma mk_env_bexp_consistent_ugt :
   forall (w : nat) (e e0 : QFBV64.exp w) (m : vm) (s : QFBV64.State.t)
@@ -11590,11 +11849,6 @@ Proof.
 Admitted.
 
 Lemma mk_env_bexp_consistent_lneg :
-  (* forall (b : QFBV64.bexp) (m : vm) (s : QFBV64.State.t) (E : env) *)
-  (*        (g : generator) (m' : vm) (E' : env) (g' : generator) *)
-  (*        (cs : cnf) (lr : literal), *)
-  (*   mk_env_bexp m s E g (QFBV64.bvLneg b) = (m', E', g', cs, lr) -> *)
-  (*   newer_than_vm g m -> consistent m E s -> consistent m' E' simpl. *)
   forall (b : QFBV64.bexp),
     (forall (m : vm) (s : QFBV64.State.t) (E : env) (g : generator)
             (m' : vm) (E' : env) (g' : generator) (cs : cnf)
@@ -11648,11 +11902,6 @@ Proof.
 Qed.
 
 Lemma mk_env_bexp_consistent_disj :
-(*  forall (b b0 : QFBV64.bexp) (m : vm) (s : QFBV64.State.t)
-         (E : env) (g : generator) (m' : vm) (E' : env) (g' : generator)
-         (cs : cnf) (lr : literal),
-    mk_env_bexp m s E g (QFBV64.bvDisj b b0) = (m', E', g', cs, lr) ->
-    newer_than_vm g m -> consistent m E s -> consistent m' E' s.*)
   forall (b : QFBV64.bexp),
     (forall (m : vm) (s : QFBV64.State.t) (E : env) (g : generator)
             (m' : vm) (E' : env) (g' : generator) (cs : cnf)
@@ -11752,9 +12001,11 @@ Proof.
     move: (mk_env_exp_consistent _ e1) (mk_env_exp_consistent _ e2) => IH1 IH2.
     exact: (mk_env_bexp_consistent_eq IH1 IH2).
   - move=> w e1 e2.
-    move: (mk_env_exp_consistent _ e1) (mk_env_exp_consistent _ e2) => IH1 IH2.
-    exact: (mk_env_bexp_consistent_ult IH1 IH2).
-  - exact: mk_env_bexp_consistent_ule.
+    move: (mk_env_exp_consistent _ e1) (mk_env_exp_consistent _ e2) => ih1 ih2.
+    exact: (mk_env_bexp_consistent_ult ih1 ih2).
+  - move=> w e1 e2.
+    move: (mk_env_exp_consistent _ e1) (mk_env_exp_consistent _ e2) => ih1 ih2.
+    exact: (mk_env_bexp_consistent_ule ih1 ih2).
   - exact: mk_env_bexp_consistent_ugt.
   - exact: mk_env_bexp_consistent_uge.
   - exact: mk_env_bexp_consistent_slt.
@@ -12268,13 +12519,32 @@ Proof.
 Qed.
 
 Lemma mk_env_bexp_preserve_ule :
-  forall (w : nat) (e e0 : QFBV64.exp w) (m : vm) (s : QFBV64.State.t)
-         (E : env) (g : generator) (m' : vm) (E' : env) (g' : generator)
-         (cs : cnf) (lr : literal),
-    mk_env_bexp m s E g (QFBV64.bvUle w e e0) = (m', E', g', cs, lr) ->
-    env_preserve E E' g.
+  forall (w : nat) (e : QFBV64.exp w),
+    (forall (m : vm) (s : QFBV64.State.t) (E : env) (g : generator)
+            (m' : vm) (E' : env) (g' : generator) (cs : cnf)
+            (lrs : w.-tuple literal),
+        mk_env_exp m s E g e = (m', E', g', cs, lrs) -> env_preserve E E' g) ->
+    forall (e0 : QFBV64.exp w),
+      (forall (m : vm) (s : QFBV64.State.t) (E : env) (g : generator)
+              (m' : vm) (E' : env) (g' : generator) (cs : cnf)
+              (lrs : w.-tuple literal),
+          mk_env_exp m s E g e0 = (m', E', g', cs, lrs) -> env_preserve E E' g) ->
+      forall (m : vm) (s : QFBV64.State.t)
+             (E : env) (g : generator) (m' : vm) (E' : env) (g' : generator)
+             (cs : cnf) (lr : literal),
+        mk_env_bexp m s E g (QFBV64.bvUle w e e0) = (m', E', g', cs, lr) ->
+        env_preserve E E' g.
 Proof.
-Admitted.
+  move=> w e1 IH1 e2 IH2 m s E g m' E' g' cs lr /=.
+  case Henv1: (mk_env_exp m s E g e1) => [[[[m1 E1] g1] cs1] ls1].
+  case Henv2: (mk_env_exp m1 s E1 g1 e2) => [[[[m2 E2] g2] cs2] ls2].
+  case Hule: (mk_env_ule E2 g2 ls1 ls2)=> [[[oE og] ocs] olr]. case=> _ <- _ _ _.
+  apply: (env_preserve_trans (IH1 _ _ _ _ _ _ _ _ _ Henv1)).
+  apply: (env_preserve_le _ (mk_env_exp_newer_gen Henv1)).
+  apply: (env_preserve_trans (IH2 _ _ _ _ _ _ _ _ _ Henv2)).
+  apply: (env_preserve_le _ (mk_env_exp_newer_gen Henv2)).
+  exact: (mk_env_ule_preserve Hule).
+Qed.
 
 Lemma mk_env_bexp_preserve_ugt :
   forall (w : nat) (e e0 : QFBV64.exp w) (m : vm) (s : QFBV64.State.t)
@@ -12385,10 +12655,6 @@ Proof.
 Admitted.
 
 Lemma mk_env_bexp_preserve_lneg :
-  (* forall (b : QFBV64.bexp) (m : vm) (s : QFBV64.State.t) (E : env) *)
-  (*        (g : generator) (m' : vm) (E' : env) (g' : generator) *)
-  (*        (cs : cnf) (lr : literal), *)
-  (*   mk_env_bexp m s E g (QFBV64.bvLneg b) = (m', E', g', cs, lr) -> env_preserve E E' g. *)
   forall (b : QFBV64.bexp),
     (forall (m : vm) (s : QFBV64.State.t) (E : env) (g : generator)
             (m' : vm) (E' : env) (g' : generator) (cs : cnf)
@@ -12442,11 +12708,6 @@ Proof.
 Qed.
 
 Lemma mk_env_bexp_preserve_disj :
-(*  forall (b b0 : QFBV64.bexp) (m : vm) (s : QFBV64.State.t)
-         (E : env) (g : generator) (m' : vm) (E' : env) (g' : generator)
-         (cs : cnf) (lr : literal),
-    mk_env_bexp m s E g (QFBV64.bvDisj b b0) = (m', E', g', cs, lr) ->
-    env_preserve E E' g.*)
   forall (b : QFBV64.bexp),
     (forall (m : vm) (s : QFBV64.State.t) (E : env) (g : generator)
             (m' : vm) (E' : env) (g' : generator) (cs : cnf)
@@ -12546,7 +12807,9 @@ Proof.
   - move=> w e1 e2.
     move: (mk_env_exp_preserve _ e1) (mk_env_exp_preserve _ e2) => IH1 IH2.
     exact: (mk_env_bexp_preserve_ult IH1 IH2).
-  - exact: mk_env_bexp_preserve_ule.
+  - move=> w e1 e2.
+    move: (mk_env_exp_preserve _ e1) (mk_env_exp_preserve _ e2) => IH1 IH2.
+    exact: (mk_env_bexp_preserve_ule IH1 IH2).
   - exact: mk_env_bexp_preserve_ugt.
   - exact: mk_env_bexp_preserve_uge.
   - exact: mk_env_bexp_preserve_slt.
@@ -13280,13 +13543,51 @@ Proof.
 Qed.
 
 Lemma mk_env_bexp_sat_ule :
-  forall (w : nat) (e e0 : QFBV64.exp w) (m : vm) (s : QFBV64.State.t)
-         (E : env) (g : generator) (m' : vm) (E' : env) (g' : generator)
-         (cs : cnf) (lr : literal),
-    mk_env_bexp m s E g (QFBV64.bvUle w e e0) = (m', E', g', cs, lr) ->
-    newer_than_vm g m -> newer_than_lit g lit_tt -> interp_cnf E' cs.
+  forall (w : nat) (e : QFBV64.exp w),
+    (forall (m : vm) (s : QFBV64.State.t) (E : env) (g : generator)
+            (m' : vm) (E' : env) (g' : generator) (cs : cnf)
+            (lrs : w.-tuple literal),
+        mk_env_exp m s E g e = (m', E', g', cs, lrs) ->
+        newer_than_vm g m -> newer_than_lit g lit_tt -> interp_cnf E' cs) ->
+    forall (e0 : QFBV64.exp w),
+      (forall (m : vm) (s : QFBV64.State.t) (E : env) (g : generator)
+              (m' : vm) (E' : env) (g' : generator) (cs : cnf)
+              (lrs : w.-tuple literal),
+          mk_env_exp m s E g e0 = (m', E', g', cs, lrs) ->
+          newer_than_vm g m -> newer_than_lit g lit_tt -> interp_cnf E' cs) ->
+      forall (m : vm) (s : QFBV64.State.t)
+             (E : env) (g : generator) (m' : vm) (E' : env) (g' : generator)
+             (cs : cnf) (lr : literal),
+        mk_env_bexp m s E g (QFBV64.bvUle w e e0) = (m', E', g', cs, lr) ->
+        newer_than_vm g m -> newer_than_lit g lit_tt -> interp_cnf E' cs.
 Proof.
-Admitted.
+  move=> w e1 IH1 e2 IH2 m s E g m' E' g' cs lr /=.
+  case Henv1: (mk_env_exp m s E g e1) => [[[[m1 E1] g1] cs1] ls1].
+  case Henv2: (mk_env_exp m1 s E1 g1 e2) => [[[[m2 E2] g2] cs2] ls2].
+  case Hule: (mk_env_ule E2 g2 ls1 ls2) => [[[oE og] ocs] olr].
+  case=> _ <- _ <- _ Hnew_gm Hnew_gtt. rewrite !interp_cnf_append.
+  move: (mk_env_exp_preserve Henv2) => Hpre_E1E2g1.
+  move: (mk_env_exp_newer_gen Henv1) => H_gg1.
+  move: (mk_env_exp_newer_gen Henv2) => H_g1g2.
+  move: (mk_env_exp_newer_cnf Henv1 Hnew_gm Hnew_gtt) => Hnew_g1cs1.
+  move: (newer_than_cnf_le_newer Hnew_g1cs1 H_g1g2) => Hnew_g2cs1.
+  move: (mk_env_exp_newer_vm Henv1 Hnew_gm) => Hnew_g1m1.
+  move: (newer_than_lit_le_newer Hnew_gtt H_gg1) => Hnew_g1tt.
+  move: (mk_env_exp_newer_cnf Henv2 Hnew_g1m1 Hnew_g1tt) => Hnew_g2cs2.
+  move: (mk_env_exp_newer_res Henv1 Hnew_gm Hnew_gtt) => Hnew_g1ls1.
+  move: (mk_env_exp_newer_res Henv2 Hnew_g1m1 Hnew_g1tt) => Hnew_g2ls2.
+  move: (newer_than_lits_le_newer Hnew_g1ls1 H_g1g2) =>
+  {H_g1g2 Hnew_g1ls1} Hnew_g2ls1.
+  (* interp_cnf oE cs1 *)
+  rewrite (env_preserve_cnf (mk_env_ule_preserve Hule) Hnew_g2cs1).
+  rewrite (env_preserve_cnf Hpre_E1E2g1 Hnew_g1cs1).
+  rewrite (IH1 _ _ _ _ _ _ _ _ _ Henv1 Hnew_gm Hnew_gtt) andTb.
+  (* interp_cnf oE cs2 *)
+  rewrite (env_preserve_cnf (mk_env_ule_preserve Hule) Hnew_g2cs2).
+  rewrite (IH2 _ _ _ _ _ _ _ _ _ Henv2 Hnew_g1m1 Hnew_g1tt) andTb.
+  (* interp_cnf oE ocs *)
+  exact: (mk_env_ule_sat Hule Hnew_g2ls1 Hnew_g2ls2).
+Qed.
 
 Lemma mk_env_bexp_sat_ugt :
   forall (w : nat) (e e0 : QFBV64.exp w) (m : vm) (s : QFBV64.State.t)
@@ -13397,11 +13698,6 @@ Proof.
 Admitted.
 
 Lemma mk_env_bexp_sat_lneg :
-  (* forall (b : QFBV64.bexp) (m : vm) (s : QFBV64.State.t) (E : env) *)
-  (*        (g : generator) (m' : vm) (E' : env) (g' : generator) *)
-  (*        (cs : cnf) (lr : literal), *)
-  (*   mk_env_bexp m s E g (QFBV64.bvLneg b) = (m', E', g', cs, lr) -> *)
-  (*   newer_than_vm g m -> newer_than_lit g lit_tt -> interp_cnf E' cs. *)
   forall (b : QFBV64.bexp),
     (forall (m : vm) (s : QFBV64.State.t) (E : env) (g : generator)
             (m' : vm) (E' : env) (g' : generator) (cs : cnf)
@@ -13477,11 +13773,6 @@ Proof.
 Qed.
 
 Lemma mk_env_bexp_sat_disj :
-(*  forall (b b0 : QFBV64.bexp) (m : vm) (s : QFBV64.State.t)
-         (E : env) (g : generator) (m' : vm) (E' : env) (g' : generator)
-         (cs : cnf) (lr : literal),
-    mk_env_bexp m s E g (QFBV64.bvDisj b b0) = (m', E', g', cs, lr) ->
-    newer_than_vm g m -> newer_than_lit g lit_tt -> interp_cnf E' cs.*)
   forall (b : QFBV64.bexp),
     (forall (m : vm) (s : QFBV64.State.t) (E : env) (g : generator)
             (m' : vm) (E' : env) (g' : generator) (cs : cnf)
@@ -13598,7 +13889,9 @@ Proof.
   - move=> w e1 e2.
     move: (mk_env_exp_sat _ e1) (mk_env_exp_sat _ e2) => IH1 IH2.
     exact: (mk_env_bexp_sat_ult IH1 IH2).
-  - exact: mk_env_bexp_sat_ule.
+  - move=> w e1 e2.
+    move: (mk_env_exp_sat _ e1) (mk_env_exp_sat _ e2) => IH1 IH2.
+    exact: (mk_env_bexp_sat_ule IH1 IH2).
   - exact: mk_env_bexp_sat_ugt.
   - exact: mk_env_bexp_sat_uge.
   - exact: mk_env_bexp_sat_slt.
